src/Analysis/Instances/Sign/Sign_Side_Soundness.thy
@@ -1,5 +1,5 @@
 theory Sign_Side_Soundness
-  imports Sign_Domain LTR_TD_Side_Eff_Exit Retain_Analysis
+  imports Sign_Domain LTR_TD_Side_Eff_Exit
 begin
 
 section \<open>Sign domain: effectful transfer instance\<close>
@@ -27,6 +27,14 @@ lemma sign_etf_combine_tree:
   "etf_combine sign_etf dst cc ex = unit_combine_tree dst cc ex"
   unfolding sign_etf_def etf_combine_mixed_of_transfer by simp
 
+lemma sign_etf_enter_tree:
+  "etf_enter sign_etf fs as cl = unit_edge_tree (tf_enter sign_tf fs as) cl"
+  unfolding sign_etf_def mixed_etf_of_transfer_def by simp
+
+lemma sign_tf_enter_mono:
+  "s1 \<le> s2 \<Longrightarrow> tf_enter sign_tf fs as s1 \<le> tf_enter sign_tf fs as s2"
+  by (simp add: sign_tf_def enter_sign_mono)
+
 lemma sign_sound_etf:
   "sound_effectful_transfer sign_etf"
   unfolding sign_etf_def
@@ -35,12 +43,13 @@ lemma sign_sound_etf:
 
 lemma sign_etf_cone_compatible: "cone_compatible_etf sign_etf"
   by (rule cone_compatible_etf_local_unit_transfer
-       [OF sign_etf_edge_tree_mixed sign_etf_combine_tree])
+       [OF sign_etf_edge_tree_mixed sign_etf_enter_tree sign_etf_combine_tree])
 
 lemma sign_etf_threefold_mono:
   "threefold_mono (side_cfg_T_eff g sign_etf bot0 s0 ())"
   by (rule threefold_mono_local_unit_transfer
-       [OF sign_etf_edge_tree_mixed sign_etf_combine_tree sign_tf_mono])
+       [OF sign_etf_edge_tree_mixed sign_etf_enter_tree sign_etf_combine_tree
+           sign_tf_mono sign_tf_enter_mono])
 
 subsection \<open>Unit-only sign ETF (executable transport)\<close>
 
@@ -61,185 +70,39 @@ lemma sign_etf_unit_combine_tree:
   "etf_combine sign_etf_unit dst cc ex = unit_combine_tree dst cc ex"
   unfolding sign_etf_unit_def etf_combine_unit_of_transfer by simp
 
+lemma sign_etf_unit_enter_tree_tf:
+  "etf_enter sign_etf_unit fs as cl = unit_edge_tree (tf_enter sign_tf fs as) cl"
+  unfolding sign_etf_unit_def unit_etf_of_transfer_def by simp
+
+lemma sign_etf_unit_enter_tree:
+  "etf_enter sign_etf_unit xs es u =
+    unit_edge_tree (\<lambda>s. bind_formals_abs xs
+      (map (\<lambda>e. aval_sign e s) es) (enter_frame_sign s)) u"
+proof -
+  have enter:
+    "enter_sign xs es = (\<lambda>s. bind_formals_abs xs
+      (map (\<lambda>e. aval_sign e s) es) (enter_frame_sign s))"
+    by (rule ext) (simp add: enter_sign_def)
+  show ?thesis
+    unfolding sign_etf_unit_def unit_etf_of_transfer_def
+    by (simp add: sign_tf_def enter)
+qed
+
 lemma sign_sound_etf_unit:
   "sound_effectful_transfer sign_etf_unit"
   unfolding sign_etf_unit_def
   by (rule sound_effectful_transfer_unit_of_transfer [OF sign_is_sound_transfer])
 
-definition sign_etf_retain :: "(unit, sign) effectful_domain_transfer" where
-  "sign_etf_retain = retain_etf_of_transfer sign_tf"
-
-lemma sign_etf_retain_edge_tree:
-  "apply_etf sign_etf_retain a u = retain_edge_tree (apply_tf sign_tf a) u"
-  unfolding sign_etf_retain_def apply_etf_retain_of_transfer by simp
-
-lemma sign_etf_retain_combine_tree:
-  "etf_combine sign_etf_retain dst cc ex = unit_combine_tree dst cc ex"
-  unfolding sign_etf_retain_def etf_combine_retain_of_transfer by simp
-
-lemma sign_sound_etf_retain:
-  "sound_effectful_transfer sign_etf_retain"
-  unfolding sign_etf_retain_def
-  by (rule sound_effectful_transfer_retain_of_transfer [OF sign_is_sound_transfer])
-
-lemma sign_etf_retain_enter:
-  "etf_enter sign_etf_retain xs es u = retain_edge_tree (tf_enter sign_tf xs es) u"
-  by (simp add: sign_etf_retain_def retain_etf_of_transfer_def)
-
-text \<open>
-  The fresh callee frame for the sign enter transfer: locals reset to @{term STop}
-  (the abstraction of the zeroed callee frame), globals bot.  It is exactly
-  @{term \<open>restrict_local (enter_frame_sign x)\<close>}, independent of the input
-  @{term x}.  Parameter binding writes locals on top of this frame, which stays
-  below it because @{term STop} is the sign top.
-\<close>
-
-definition fresh_frame_sign :: "sign abs_state" where
-  "fresh_frame_sign = (\<lambda>x. if is_global x then \<bottom> else STop)"
-
-lemma sign_le_STop [simp]: "(a::sign) \<le> STop"
-  by (cases a) (simp_all add: less_eq_sign_def)
-
-lemma sign_etf_unit_enter:
-  "etf_enter sign_etf_unit xs es u = unit_edge_tree (tf_enter sign_tf xs es) u"
-  by (simp add: sign_etf_unit_def unit_etf_of_transfer_def)
-
-lemma sign_sound_etf_unit_framed:
-  "sound_effectful_transfer_framed sign_etf_unit fresh_frame_sign"
-proof (rule sound_effectful_transfer_framed.intro)
-  show "sound_effectful_transfer sign_etf_unit" by (rule sign_sound_etf_unit)
-next
-  show "sound_effectful_transfer_framed_axioms sign_etf_unit fresh_frame_sign"
-    unfolding sound_effectful_transfer_framed_axioms_def
-  proof (intro allI impI)
-    fix xs and es :: "aexp list" and u and \<sigma> :: "pp + unit \<Rightarrow> sign abs_state"
-    assume loc: "local_formals xs"
-    assume inr: "inr_slot_locals_bot \<sigma>" and inl: "inl_slot_globals_bot \<sigma>"
-    have "etf_full (etf_enter sign_etf_unit xs es u) \<sigma>
-            = enter_sign xs es (\<sigma> (Inl u) \<squnion> \<sigma> (Inr ()))"
-      by (simp add: sign_etf_unit_enter etf_full_unit_edge_tree sign_tf_def)
-    also have "\<dots> \<le> fresh_frame_sign \<squnion> glob_env \<sigma>"
-    proof (rule le_funI)
-      fix x
-      show "enter_sign xs es (\<sigma> (Inl u) \<squnion> \<sigma> (Inr ())) x
-              \<le> (fresh_frame_sign \<squnion> glob_env \<sigma>) x"
-      proof (cases "is_global x")
-        case True
-        \<comment> \<open>Formals are local, so a global slot survives the binding untouched.\<close>
-        have "enter_sign xs es (\<sigma> (Inl u) \<squnion> \<sigma> (Inr ())) x
-                = enter_frame_sign (\<sigma> (Inl u) \<squnion> \<sigma> (Inr ())) x"
-          unfolding enter_sign_def by (rule bind_formals_abs_global[OF loc True])
-        moreover have "\<sigma> (Inl u) x = \<bottom>"
-          using inl True by (simp add: inl_slot_globals_bot_def)
-        ultimately show ?thesis using True
-          by (simp add: enter_frame_sign_def fresh_frame_sign_def glob_env_unit)
-      next
-        case False
-        \<comment> \<open>A local slot is bounded by the fresh frame's \<open>STop\<close>, the sign top.\<close>
-        show ?thesis using False
-          by (simp add: fresh_frame_sign_def le_supI1)
-      qed
-    qed
-    finally show "etf_full (etf_enter sign_etf_unit xs es u) \<sigma>
-                    \<le> fresh_frame_sign \<squnion> glob_env \<sigma>" .
-  qed
-qed
-
-text \<open>
-  Retain companion: the enter bound also holds under the weaker
-  @{const inl_glob_le_glob_env} premise, so the retain Sign spine (local slots
-  carrying globals) discharges the framed contract.  Same proof, but the global
-  case bounds @{term "\<sigma> (Inl u) x"} by @{const glob_env} rather than forcing it to
-  @{term \<bottom>}.
-\<close>
-lemma sign_sound_etf_unit_framed_le:
-  "sound_effectful_transfer_framed_le sign_etf_unit fresh_frame_sign"
-proof (rule sound_effectful_transfer_framed_le.intro)
-  show "sound_effectful_transfer sign_etf_unit" by (rule sign_sound_etf_unit)
-next
-  show "sound_effectful_transfer_framed_le_axioms sign_etf_unit fresh_frame_sign"
-    unfolding sound_effectful_transfer_framed_le_axioms_def
-  proof (intro allI impI)
-    fix xs and es :: "aexp list" and u and \<sigma> :: "pp + unit \<Rightarrow> sign abs_state"
-    assume loc: "local_formals xs"
-    assume inr: "inr_slot_locals_bot \<sigma>" and inl: "inl_glob_le_glob_env \<sigma>"
-    have "etf_full (etf_enter sign_etf_unit xs es u) \<sigma>
-            = enter_sign xs es (\<sigma> (Inl u) \<squnion> \<sigma> (Inr ()))"
-      by (simp add: sign_etf_unit_enter etf_full_unit_edge_tree sign_tf_def)
-    also have "\<dots> \<le> fresh_frame_sign \<squnion> glob_env \<sigma>"
-    proof (rule le_funI)
-      fix x
-      show "enter_sign xs es (\<sigma> (Inl u) \<squnion> \<sigma> (Inr ())) x
-              \<le> (fresh_frame_sign \<squnion> glob_env \<sigma>) x"
-      proof (cases "is_global x")
-        case True
-        have "enter_sign xs es (\<sigma> (Inl u) \<squnion> \<sigma> (Inr ())) x
-                = enter_frame_sign (\<sigma> (Inl u) \<squnion> \<sigma> (Inr ())) x"
-          unfolding enter_sign_def by (rule bind_formals_abs_global[OF loc True])
-        moreover have "\<sigma> (Inl u) x \<le> glob_env \<sigma> x"
-          using inl True by (simp add: inl_glob_le_glob_env_def)
-        ultimately show ?thesis using True
-          by (simp add: enter_frame_sign_def fresh_frame_sign_def glob_env_unit
-                sup_fun_def le_sup_iff)
-      next
-        case False
-        show ?thesis using False
-          by (simp add: fresh_frame_sign_def le_supI1)
-      qed
-    qed
-    finally show "etf_full (etf_enter sign_etf_unit xs es u) \<sigma>
-                    \<le> fresh_frame_sign \<squnion> glob_env \<sigma>" .
-  qed
-qed
-
-lemma sign_sound_etf_retain_framed_le:
-  "sound_effectful_transfer_framed_le sign_etf_retain fresh_frame_sign"
-proof (rule sound_effectful_transfer_framed_le.intro)
-  show "sound_effectful_transfer sign_etf_retain" by (rule sign_sound_etf_retain)
-next
-  show "sound_effectful_transfer_framed_le_axioms sign_etf_retain fresh_frame_sign"
-    unfolding sound_effectful_transfer_framed_le_axioms_def
-  proof (intro allI impI)
-    fix xs and es :: "aexp list" and u and \<sigma> :: "pp + unit \<Rightarrow> sign abs_state"
-    assume loc: "local_formals xs"
-    assume inr: "inr_slot_locals_bot \<sigma>" and inl: "inl_glob_le_glob_env \<sigma>"
-    have "etf_full (etf_enter sign_etf_retain xs es u) \<sigma>
-            = enter_sign xs es (\<sigma> (Inl u) \<squnion> \<sigma> (Inr ()))"
-      by (simp add: sign_etf_retain_enter etf_full_retain_edge_tree sign_tf_def)
-    also have "\<dots> \<le> fresh_frame_sign \<squnion> glob_env \<sigma>"
-    proof (rule le_funI)
-      fix x
-      show "enter_sign xs es (\<sigma> (Inl u) \<squnion> \<sigma> (Inr ())) x
-              \<le> (fresh_frame_sign \<squnion> glob_env \<sigma>) x"
-      proof (cases "is_global x")
-        case True
-        have "enter_sign xs es (\<sigma> (Inl u) \<squnion> \<sigma> (Inr ())) x
-                = enter_frame_sign (\<sigma> (Inl u) \<squnion> \<sigma> (Inr ())) x"
-          unfolding enter_sign_def by (rule bind_formals_abs_global[OF loc True])
-        moreover have "\<sigma> (Inl u) x \<le> glob_env \<sigma> x"
-          using inl True by (simp add: inl_glob_le_glob_env_def)
-        ultimately show ?thesis using True
-          by (simp add: enter_frame_sign_def fresh_frame_sign_def glob_env_unit
-                sup_fun_def le_sup_iff)
-      next
-        case False
-        show ?thesis using False
-          by (simp add: fresh_frame_sign_def le_supI1)
-      qed
-    qed
-    finally show "etf_full (etf_enter sign_etf_retain xs es u) \<sigma>
-                    \<le> fresh_frame_sign \<squnion> glob_env \<sigma>" .
-  qed
-qed
 
 lemma sign_etf_unit_cone_compatible: "cone_compatible_etf sign_etf_unit"
   by (rule cone_compatible_etf_unit_transfer
-       [OF sign_etf_unit_edge_tree sign_etf_unit_combine_tree])
+       [OF sign_etf_unit_edge_tree sign_etf_unit_enter_tree_tf sign_etf_unit_combine_tree])
 
 lemma sign_etf_unit_threefold_mono:
   "threefold_mono (side_cfg_T_eff g sign_etf_unit bot0 s0 ())"
   by (rule threefold_mono_unit_transfer
-       [OF sign_etf_unit_edge_tree sign_etf_unit_combine_tree sign_tf_mono])
+       [OF sign_etf_unit_edge_tree sign_etf_unit_enter_tree_tf sign_etf_unit_combine_tree
+           sign_tf_mono sign_tf_enter_mono])
 
 section \<open>Sign domain: standalone effectful interprocedural soundness\<close>
 
@@ -251,23 +114,23 @@ text \<open>
 \<close>
 
 theorem side_sign_analysis_sound:
-  fixes \<Pi> ps main and s t :: store and s0 :: "sign abs_state"
+  fixes \<Pi> ps mnm main and s t :: store and s0 :: "sign abs_state"
   assumes s_sound: "s \<in> \<lbrakk>s0\<rbrakk>"
   assumes collect_exit:
-    "t \<in> ltr_collect (compile_prog \<Pi> ps main) {s}
-       (cfg_exit (compile_prog \<Pi> ps main))"
+    "t \<in> ltr_collect (compile_prog \<Pi> ps mnm main) {s}
+       (cfg_exit (compile_prog \<Pi> ps mnm main))"
   assumes side_solve_dom:
-    "side_cfg_solve_dom_eff (compile_prog \<Pi> ps main) sign_etf bot s0 ()
-       (cfg_exit (compile_prog \<Pi> ps main))"
-  shows "t \<in> \<lbrakk>side_analyse_eff \<Pi> ps main sign_etf bot s0 ()
-         (cfg_exit (compile_prog \<Pi> ps main))\<rbrakk>"
+    "side_cfg_solve_dom_eff (compile_prog \<Pi> ps mnm main) sign_etf bot s0 ()
+       (cfg_exit (compile_prog \<Pi> ps mnm main))"
+  shows "t \<in> \<lbrakk>side_analyse_eff \<Pi> ps mnm main sign_etf bot s0 ()
+         (cfg_exit (compile_prog \<Pi> ps mnm main))\<rbrakk>"
 proof -
   have gs: "{s} \<le> \<lbrakk>s0\<rbrakk>" using s_sound by simp
   have collect:
-    "ltr_collect (compile_prog \<Pi> ps main) {s}
-       (cfg_exit (compile_prog \<Pi> ps main))
-     \<le> \<lbrakk>side_analyse_eff \<Pi> ps main sign_etf bot s0 ()
-           (cfg_exit (compile_prog \<Pi> ps main))\<rbrakk>"
+    "ltr_collect (compile_prog \<Pi> ps mnm main) {s}
+       (cfg_exit (compile_prog \<Pi> ps mnm main))
+     \<le> \<lbrakk>side_analyse_eff \<Pi> ps mnm main sign_etf bot s0 ()
+           (cfg_exit (compile_prog \<Pi> ps mnm main))\<rbrakk>"
     by (rule side_analyse_eff_collect_sound_exit_ltr_cone
           [OF sign_sound_etf sign_etf_threefold_mono sign_etf_cone_compatible
               side_solve_dom gs])
@@ -275,3 +138,5 @@ proof -
 qed
 
 end
+
+
